Functional codegen for datatypes

Source/DafnyCore/Compilers/Dafny/ASTBuilder.cs
@@ -150,8 +150,8 @@ namespace Microsoft.Dafny.Compilers {
     DafnyCompiler compiler { get; }
     void AddDatatype(Datatype item);
 
-    public DatatypeBuilder Datatype(string name) {
-      return new DatatypeBuilder(this, name);
+    public DatatypeBuilder Datatype(string name, List<DAST.DatatypeCtor> ctors) {
+      return new DatatypeBuilder(this, name, ctors);
     }
   }
 
@@ -159,12 +159,13 @@ namespace Microsoft.Dafny.Compilers {
     public DafnyCompiler compiler { get => parent.compiler; }
     readonly DatatypeContainer parent;
     readonly string name;
-    // readonly List<?> ctors = new();
+    readonly List<DAST.DatatypeCtor> ctors;
     readonly List<ClassItem> body = new();
 
-    public DatatypeBuilder(DatatypeContainer parent, string name) {
+    public DatatypeBuilder(DatatypeContainer parent, string name, List<DAST.DatatypeCtor> ctors) {
       this.parent = parent;
       this.name = name;
+      this.ctors = ctors;
     }
 
     public void AddMethod(DAST.Method item) {
@@ -180,7 +181,11 @@ namespace Microsoft.Dafny.Compilers {
     }
 
     public object Finish() {
-      parent.AddDatatype((Datatype)Datatype.create(Sequence<Rune>.UnicodeFromString(this.name), Sequence<ClassItem>.FromArray(body.ToArray())));
+      parent.AddDatatype((Datatype)Datatype.create(
+        Sequence<Rune>.UnicodeFromString(this.name),
+        Sequence<DAST.DatatypeCtor>.FromArray(ctors.ToArray()),
+        Sequence<ClassItem>.FromArray(body.ToArray())
+      ));
       return parent;
     }
   }
